Good progress on finishing the new HoC

state/HigherOrderContracts.fst
@@ -7,317 +7,305 @@ open SharedRefs
 
 open Witnessable
 open TargetLang
-
-type err =
-| Contract_failure : string -> err
-
-instance witnessable_err : witnessable err = {
-  satisfy = (fun _ _ -> True);
-}
+open SpecTree
 
 instance targetlang_err pspec : targetlang pspec err = {
   wt = witnessable_err
 }
 
-type resexn a = either a err
-
-type cb_check pspec (t1:Type) (t2:Type) {| c2: witnessable t2 |}
-  (pre:(t1 -> st_pre))
-  (post:(x:t1 -> h0:heap -> st_post' t2 (pre x h0)))
-  (x:t1)
-  (eh0:FStar.Ghost.erased heap{pre x eh0}) =
-  (r:t2 -> ST (resexn unit) (fun h1 -> post_targetlang_arrow pspec eh0 r h1) (fun h1 rck h1' ->
-    h1 == h1' /\ (Inl? rck ==> post x eh0 r h1)))
-
-type select_check
-  pspec
-  (t1:Type) (t2:Type) {| c2: witnessable t2 |}
-  (pre:(t1 -> st_pre))
-  (post:(x:t1 -> h0:heap -> st_post' t2 (pre x h0))) =
-  x:t1 -> ST (
-    eh0:FStar.Ghost.erased heap{pre x eh0} & cb_check pspec t1 t2 #c2 pre post x eh0
-  ) (pre x) (fun h0 r h1 -> FStar.Ghost.reveal (dfst r) == h0 /\ h0 == h1)
-
-class exportable_from pspec (styp: Type u#a) = {
+class exportable_from pspec (styp: Type u#a) (st:spec_tree pspec) = {
   [@@@no_method] c_styp : witnessable styp;
   [@@@no_method] ityp : Type u#b;
   [@@@no_method] c_ityp : targetlang pspec ityp;
-  [@@@no_method] export : styp -> ityp;
-  [@@@no_method] lemma_export_preserves_prref : x:styp -> prref:mref_pred -> Lemma (requires (c_styp.satisfy x prref)) (ensures (c_ityp.wt.satisfy (export x) (prref)))
+  [@@@no_method] export : hoc_tree st -> styp -> ityp;
+  [@@@no_method] lemma_export_preserves_prref :
+    x:styp -> prref:mref_pred -> hocs:hoc_tree st -> Lemma (requires (c_styp.satisfy x prref)) (ensures (c_ityp.wt.satisfy (export hocs x) (prref)))
 }
 
-class safe_importable_to pspec (styp: Type u#a) = {
+class safe_importable_to pspec (styp: Type u#a) (st:spec_tree pspec) = {
   [@@@no_method] c_styp : witnessable styp;
   [@@@no_method] ityp : Type u#b;
   [@@@no_method] c_ityp : targetlang pspec ityp;
-  [@@@no_method] safe_import : ityp -> styp;
-  [@@@no_method] lemma_safe_import_preserves_prref : x:ityp -> prref:mref_pred -> Lemma (requires (c_ityp.wt.satisfy x (prref))) (ensures (c_styp.satisfy (safe_import x) (prref)))
+  [@@@no_method] safe_import : ityp -> hoc_tree st -> styp;
+  [@@@no_method] lemma_safe_import_preserves_prref :
+    x:ityp -> prref:mref_pred -> hocs:hoc_tree st -> Lemma (requires (c_ityp.wt.satisfy x (prref))) (ensures (c_styp.satisfy (safe_import x hocs) (prref)))
 }
 
-class importable_to pspec (styp: Type u#a) = {
+class importable_to pspec (styp: Type u#a) (st:spec_tree pspec) = {
   [@@@no_method] c_styp : witnessable styp;
   [@@@no_method] ityp : Type u#b;
   [@@@no_method] c_ityp : targetlang pspec ityp;
-  [@@@no_method] import : ityp -> resexn styp;
-  [@@@no_method] lemma_import_preserves_prref : x:ityp -> prref:mref_pred -> Lemma (requires (c_ityp.wt.satisfy x prref)) (ensures ((witnessable_sum styp err).satisfy (import x) prref))
+  [@@@no_method] import : ityp -> hoc_tree st -> resexn styp;
+  [@@@no_method] lemma_import_preserves_prref :
+    x:ityp -> prref:mref_pred -> hocs:hoc_tree st -> Lemma (requires (c_ityp.wt.satisfy x prref)) (ensures ((witnessable_sum styp err).satisfy (import x hocs) prref))
 }
 
 (** Exportable instances **)
-instance targetlang_is_exportable t pspec {| c1:targetlang pspec t |} : exportable_from pspec t = {
+instance targetlang_is_exportable t pspec {| c1:targetlang pspec t |} : exportable_from pspec t Leaf = {
   c_styp = c1.wt;
   ityp = t;
   c_ityp = solve;
-  export = (fun x -> x);
-  lemma_export_preserves_prref = (fun _ _ -> ()) }
+  export = (fun Leaf x -> x);
+  lemma_export_preserves_prref = (fun _ _ _ -> ()) }
 
-instance exportable_unit pspec : exportable_from pspec unit = {
+instance exportable_unit pspec : exportable_from pspec unit Leaf = {
   c_styp = witnessable_unit;
   ityp = unit;
   c_ityp = targetlang_unit _;
-  export = (fun x -> x);
-  lemma_export_preserves_prref = (fun _ _ -> ())
+  export = (fun Leaf x -> x);
+  lemma_export_preserves_prref = (fun _ _ _ -> ())
 }
 
-instance exportable_err pspec : exportable_from pspec err = {
+instance exportable_err pspec : exportable_from pspec err Leaf = {
   c_styp = witnessable_err;
   ityp = err;
   c_ityp = targetlang_err _;
-  export = (fun x -> x);
-  lemma_export_preserves_prref = (fun _ _ -> ())
+  export = (fun Leaf x -> x);
+  lemma_export_preserves_prref = (fun _ _ _ -> ())
 }
 
-instance exportable_int pspec : exportable_from pspec int = {
+instance exportable_int pspec : exportable_from pspec int Leaf = {
   c_styp = witnessable_int;
   ityp = int;
   c_ityp = targetlang_int _;
-  export = (fun x -> x);
-  lemma_export_preserves_prref = (fun _ _ -> ())
+  export = (fun Leaf x -> x);
+  lemma_export_preserves_prref = (fun _ _ _ -> ())
 }
 
-instance exportable_option pspec t {| c:exportable_from pspec t |} : exportable_from pspec (option t) = {
+instance exportable_option pspec t specs {| c:exportable_from pspec t specs |} : exportable_from pspec (option t) specs = {
   c_styp = witnessable_option t #c.c_styp;
   ityp = option c.ityp;
   c_ityp = targetlang_option _ c.ityp #c.c_ityp;
-  export = (fun x -> match x with | Some x -> Some (c.export x) | None -> None);
-  lemma_export_preserves_prref = (fun x p -> match x with | Some x -> c.lemma_export_preserves_prref x p | None -> ())
+  export = (fun hocs x -> match x with | Some x -> Some (c.export hocs x) | None -> None);
+  lemma_export_preserves_prref = (fun x p hocs -> match x with | Some x -> c.lemma_export_preserves_prref x p hocs | None -> ())
 }
 
-instance exportable_sum pspec t1 t2 {| c1:exportable_from pspec t1 |} {| c2:exportable_from pspec t2 |} : exportable_from pspec (either t1 t2) = {
+instance exportable_sum pspec t1 t2 s1 s2 {| c1:exportable_from pspec t1 s1 |} {| c2:exportable_from pspec t2 s2 |} : exportable_from pspec (either t1 t2) (EmptyNode s1 s2) = {
   c_styp = witnessable_sum t1 t2 #c1.c_styp #c2.c_styp;
   ityp = either c1.ityp c2.ityp;
   c_ityp = targetlang_sum _ _ _ #c1.c_ityp #c2.c_ityp;
-  export = (fun x -> match x with | Inl x -> Inl (c1.export x) | Inr x -> Inr (c2.export x));
-  lemma_export_preserves_prref = (fun x ->
-    match x with | Inl x -> c1.lemma_export_preserves_prref x | Inr x -> c2.lemma_export_preserves_prref x)
+  export = (fun hocs x -> match x with | Inl x -> Inl (c1.export (left hocs) x) | Inr x -> Inr (c2.export (right hocs) x));
+  lemma_export_preserves_prref = (fun x p hocs ->
+    match x with | Inl x -> c1.lemma_export_preserves_prref x p (left hocs)| Inr x -> c2.lemma_export_preserves_prref x p (right hocs))
 }
 
-instance exportable_resexn pspec t {| c:exportable_from pspec t |} : exportable_from pspec (resexn t) = {
-  c_styp = witnessable_sum t err #c.c_styp;
-  ityp = resexn c.ityp;
-  c_ityp = targetlang_sum _ c.ityp err #c.c_ityp;
-  export = (fun x -> match x with | Inl x -> Inl (c.export x) | Inr err -> Inr err);
-  lemma_export_preserves_prref = (fun x p -> match x with | Inl x -> c.lemma_export_preserves_prref x p | Inr err -> ())
-}
+instance exportable_resexn pspec t spec {| c:exportable_from pspec t spec |} : exportable_from pspec (resexn t) (EmptyNode spec Leaf) =
+  exportable_sum pspec t err spec Leaf #c #(exportable_err pspec)
 
-instance exportable_pair pspec t1 t2 {| c1:exportable_from pspec t1 |} {| c2:exportable_from pspec t2 |} : exportable_from pspec (t1 * t2) = {
+instance exportable_pair pspec t1 t2 s1 s2 {| c1:exportable_from pspec t1 s1 |} {| c2:exportable_from pspec t2 s2 |} : exportable_from pspec (t1 * t2) (EmptyNode s1 s2) = {
   c_styp = witnessable_pair t1 t2 #c1.c_styp #c2.c_styp;
   ityp = c1.ityp * c2.ityp;
   c_ityp = targetlang_pair _ _ _ #c1.c_ityp #c2.c_ityp;
-  export = (fun (x1, x2) -> (c1.export x1, c2.export x2));
-  lemma_export_preserves_prref = (fun (x1, x2) p -> c1.lemma_export_preserves_prref x1 p; c2.lemma_export_preserves_prref x2 p)
+  export = (fun hocs (x1, x2) -> (c1.export (left hocs) x1, c2.export (right hocs) x2));
+  lemma_export_preserves_prref = (fun (x1, x2) p hocs -> c1.lemma_export_preserves_prref x1 p (left hocs); c2.lemma_export_preserves_prref x2 p (right hocs))
 }
 
-instance exportable_ref pspec t {| c:tc_shareable_type t |} : exportable_from pspec (ref t) = {
+instance exportable_ref pspec t {| c:tc_shareable_type t |} : exportable_from pspec (ref t) Leaf = {
   c_styp = witnessable_mref t _ #solve;
   ityp = ref t;
   c_ityp = targetlang_ref _ t #c;
-  export = (fun x -> x);
-  lemma_export_preserves_prref = (fun _ _ -> ());
+  export = (fun Leaf x -> x);
+  lemma_export_preserves_prref = (fun _ _ _ -> ());
 }
 
-instance exportable_llist pspec t {| c:exportable_from pspec t |} : exportable_from pspec (linkedList t) = admit ()
+instance exportable_llist pspec t {| c:tc_shareable_type t |} : exportable_from pspec (linkedList t) Leaf = admit ()
 
-instance exportable_refinement pspec t {| c:exportable_from pspec t |} (p:t->Type0) : exportable_from pspec (x:t{p x}) = {
+instance exportable_refinement pspec t spec {| c:exportable_from pspec t spec |} (p:t->Type0) : exportable_from pspec (x:t{p x}) spec = {
   c_styp = witnessable_refinement t #c.c_styp p;
   ityp = c.ityp;
   c_ityp = c.c_ityp;
-  export = (fun x -> c.export x);
+  export = (fun hocs x -> c.export hocs x);
   lemma_export_preserves_prref = (fun x -> c.lemma_export_preserves_prref x);
 }
 
 instance exportable_arrow
   pspec
   (t1:Type) (t2:Type)
-  {| c1:importable_to pspec t1 |}
-  {| c2:exportable_from pspec t2 |}
+  s1 s2
+  {| c1:importable_to pspec t1 s1 |}
+  {| c2:exportable_from pspec t2 s2 |}
   (pre:(t1 -> st_pre))
   (post:(x:t1 -> h0:heap -> st_post' (resexn t2) (pre x h0)))
-  (_:squash (forall x h0 r h1. post x h0 r h1 ==> post_targetlang_arrow pspec #(resexn t2) #(witnessable_sum t2 err #c2.c_styp) h0 r h1))
-  (check:select_check pspec t1 unit (pre_targetlang_arrow pspec #_ #c1.c_styp)
-    (fun x _ _ h1 -> pre x h1))
+ // (_:squash (forall x h0 r h1. post x h0 r h1 ==> post_targetlang_arrow pspec #(resexn t2) #(witnessable_sum t2 err #c2.c_styp) h0 r h1))
+ // (check:select_check pspec t1 unit (pre_targetlang_arrow pspec #_ #c1.c_styp)
+ //   (fun x _ _ h1 -> pre x h1))
                 (** ^ the fact that the check has a pre-condition means that the check does not have to enforce it
                       e.g., the invariant on the heap **)
-  : exportable_from pspec (x:t1 -> ST (resexn t2) (pre x) (post x)) = {
+  : exportable_from pspec (x:t1 -> ST (resexn t2) (pre x) (post x))
+    (Node (Spec t1 c1.c_styp pre t2 c2.c_styp post) s1 s2) = {
   c_styp = witnessable_arrow t1 (resexn t2) pre post;
-  ityp = mk_targetlang_arrow pspec c1.ityp #c1.c_ityp.wt (resexn c2.ityp) #(witnessable_sum c2.ityp err #c2.c_ityp.wt);
+  ityp = mk_targetlang_arrow pspec c1.ityp #c1.c_ityp.wt (resexn c2.ityp) #(witnessable_resexn #c2.ityp #c2.c_ityp.wt);
   c_ityp = targetlang_arrow pspec c1.ityp (resexn c2.ityp) #c1.c_ityp #(targetlang_sum pspec c2.ityp err #c2.c_ityp) ;
-  export = (fun (f:(x:t1 -> ST (resexn t2) (pre x) (post x))) (x:c1.ityp) ->
-    match c1.import x with
-    | Inl x' -> begin
-      c1.lemma_import_preserves_prref x (Mktuple3?._2 pspec);
-      let (| _, cb_check |) = check x' in
-      match cb_check () with
-      | Inl _ -> begin
-        let res = f x' in
-        (exportable_resexn pspec t2).lemma_export_preserves_prref res (Mktuple3?._2 pspec);
-        (exportable_resexn pspec t2).export res
+  export = (fun (hocs:hoc_tree _) (f:(x:t1 -> ST (resexn t2) (pre x) (post x))) (x:c1.ityp) ->
+    let Node (| _, myhoc |) lhs rhs : hoc_tree _ = hocs in
+    match myhoc with
+    | EnforcePre check c_post -> begin
+      match c1.import x lhs with
+      | Inl x' -> begin
+        c1.lemma_import_preserves_prref x (Mktuple3?._2 pspec) lhs;
+        let (| _, cb_check |) = check x' in
+        match cb_check () with
+        | Inl _ -> begin
+          let res : resexn t2 = f x' in
+          c_post x' res;
+          (exportable_resexn pspec t2 s2).lemma_export_preserves_prref res (Mktuple3?._2 pspec) (EmptyNode rhs Leaf);
+          (exportable_resexn pspec t2 s2).export (EmptyNode rhs Leaf) res
+        end
+        | Inr err -> Inr err
       end
       | Inr err -> Inr err
     end
-    | Inr err -> Inr err
+    | EnforcePost _ _ _ -> Inr (Contract_failure "Wrong contract") (** TODO: get rid off! **)
   );
-  lemma_export_preserves_prref = (fun _ _ -> ());
+  lemma_export_preserves_prref = (fun _ _ _ -> ());
 }
 
 (** Importable instances **)
-instance targetlang_is_safely_importable pspec t {| c1:targetlang pspec t |} : safe_importable_to pspec t = {
+instance targetlang_is_safely_importable pspec t {| c1:targetlang pspec t |} : safe_importable_to pspec t Leaf = {
   c_styp = c1.wt;
   ityp = t;
   c_ityp = solve;
-  safe_import = (fun x -> x);
-  lemma_safe_import_preserves_prref = (fun _ _ -> ())
+  safe_import = (fun x Leaf -> x);
+  lemma_safe_import_preserves_prref = (fun _ _ _ -> ())
 }
 
-instance safe_importable_is_importable pspec t {| c1:safe_importable_to pspec t |} : importable_to pspec t = {
+instance safe_importable_is_importable pspec t spec {| c1:safe_importable_to pspec t spec |} : importable_to pspec t spec = {
   c_styp = c1.c_styp;
   ityp = c1.ityp;
   c_ityp = c1.c_ityp;
-  import = (fun x -> Inl (c1.safe_import x));
+  import = (fun x hocs -> Inl (c1.safe_import x hocs));
   lemma_import_preserves_prref = (fun x -> c1.lemma_safe_import_preserves_prref x);
 }
 
-instance safe_importable_unit pspec : safe_importable_to pspec unit = {
+instance safe_importable_unit pspec : safe_importable_to pspec unit Leaf = {
   c_styp = witnessable_unit;
   ityp = unit;
   c_ityp = targetlang_unit _;
-  safe_import = (fun x -> x);
-  lemma_safe_import_preserves_prref = (fun _ _ -> ())
+  safe_import = (fun x Leaf -> x);
+  lemma_safe_import_preserves_prref = (fun _ _ _ -> ())
 }
 
-instance safe_importable_err pspec : safe_importable_to pspec err = {
+instance safe_importable_err pspec : safe_importable_to pspec err Leaf = {
   c_styp = witnessable_err;
   ityp = err;
   c_ityp = targetlang_err _;
-  safe_import = (fun x -> x);
-  lemma_safe_import_preserves_prref = (fun _ _ -> ())
+  safe_import = (fun x Leaf -> x);
+  lemma_safe_import_preserves_prref = (fun _ _ _ -> ())
 }
 
-instance importable_option pspec t {| c:importable_to pspec t |} : importable_to pspec (option t) = {
+instance importable_option pspec t spec {| c:importable_to pspec t spec |} : importable_to pspec (option t) spec = {
   c_styp = witnessable_option t #c.c_styp;
   ityp = option c.ityp;
   c_ityp = targetlang_option _ c.ityp #c.c_ityp;
-  import = (fun x ->
+  import = (fun x hocs ->
     match x with
     | Some x -> begin
-      match c.import x with
+      match c.import x hocs with
       | Inl x -> Inl (Some x)
       | Inr err -> Inr err
     end
     | None -> Inl None);
-  lemma_import_preserves_prref = (fun x p ->
+  lemma_import_preserves_prref = (fun x p hocs ->
     match x with
-    | Some x -> c.lemma_import_preserves_prref x p
+    | Some x -> c.lemma_import_preserves_prref x p hocs
     | None -> ())
 }
 
-instance importable_sum pspec t1 t2 {| c1:importable_to pspec t1 |} {| c2:importable_to pspec t2 |} : importable_to pspec (either t1 t2) = {
+instance importable_sum pspec t1 t2 s1 s2 {| c1:importable_to pspec t1 s1 |} {| c2:importable_to pspec t2 s2 |} : importable_to pspec (either t1 t2) (EmptyNode s1 s2) = {
   c_styp = witnessable_sum t1 t2 #c1.c_styp #c2.c_styp;
   ityp = either c1.ityp c2.ityp;
   c_ityp = targetlang_sum _ _ _ #c1.c_ityp #c2.c_ityp;
-  import = (fun x ->
+  import = (fun x hocs ->
     match x with
     | Inl x -> begin
-      match c1.import x with
+      match c1.import x (left hocs) with
       | Inl x -> Inl (Inl x)
       | Inr err -> Inr err
     end
     | Inr x -> begin
-      match c2.import x with
+      match c2.import x (right hocs) with
       | Inl x -> Inl (Inr x)
       | Inr err -> Inr err
     end);
-  lemma_import_preserves_prref = (fun x p ->
+  lemma_import_preserves_prref = (fun x p hocs ->
     match x with
-    | Inl x -> c1.lemma_import_preserves_prref x p
-    | Inr x -> c2.lemma_import_preserves_prref x p)
+    | Inl x -> c1.lemma_import_preserves_prref x p (left hocs)
+    | Inr x -> c2.lemma_import_preserves_prref x p (right hocs))
 }
 
-instance safe_importable_ref pspec t {| c:tc_shareable_type t |} : safe_importable_to pspec (ref t) = {
+instance safe_importable_ref pspec t {| c:tc_shareable_type t |} : safe_importable_to pspec (ref t) Leaf = {
   c_styp = witnessable_mref t _ #solve;
   ityp = ref t;
   c_ityp = targetlang_ref _ t;
-  safe_import = (fun x -> x);
-  lemma_safe_import_preserves_prref = (fun _ _ -> ())
+  safe_import = (fun x Leaf -> x);
+  lemma_safe_import_preserves_prref = (fun _ _ _ -> ())
 }
 
-instance importable_llits pspec t {| c:importable_to pspec t |} : importable_to pspec (linkedList t) = admit ()
+instance importable_llits pspec t {| c:tc_shareable_type t |} : importable_to pspec (linkedList t) Leaf = admit ()
 
-instance import_refinement pspec t {| c:importable_to pspec t |} (p:t->Type0) (check:(x:t -> r:bool{r ==> p x})): importable_to pspec (x:t{p x}) = {
+instance import_refinement pspec t spec {| c:importable_to pspec t spec |} (p:t->Type0) (check:(x:t -> r:bool{r ==> p x})): importable_to pspec (x:t{p x}) spec = {
   c_styp = witnessable_refinement t #c.c_styp p;
   ityp = c.ityp;
   c_ityp = c.c_ityp;
-  import = (fun x ->
-    match (c.import x) with
+  import = (fun x hocs ->
+    match (c.import x hocs) with
     | Inl x -> if check x then Inl x else Inr (Contract_failure "check of refinement failed")
     | Inr err -> Inr err);
   lemma_import_preserves_prref = (fun x -> c.lemma_import_preserves_prref x);
 }
 
-instance safe_importable_resexn pspec t {| c:importable_to pspec t |} : safe_importable_to pspec (resexn t) = {
+instance safe_importable_resexn pspec t s {| c:importable_to pspec t s |} : safe_importable_to pspec (resexn t) (EmptyNode s Leaf)= {
   c_styp = witnessable_sum t err #c.c_styp;
   ityp = resexn c.ityp;
   c_ityp = targetlang_sum _ c.ityp err #c.c_ityp;
-  safe_import = (fun x ->
+  safe_import = (fun x hocs ->
     match x with
     | Inl x -> begin
-      match c.import x with
+      match c.import x (left hocs) with
       | Inl x -> Inl x
       | Inr err -> Inr err
     end
     | Inr err -> Inr err
     );
-  lemma_safe_import_preserves_prref = (fun x p ->
+  lemma_safe_import_preserves_prref = (fun x p hocs ->
     match x with
-    | Inl x -> c.lemma_import_preserves_prref x p
+    | Inl x -> c.lemma_import_preserves_prref x p (left hocs)
     | Inr err -> ())
 }
 
 instance safe_importable_arrow
   pspec
   (t1:Type) (t2:Type)
-  {| c1:exportable_from pspec t1 |}
-  {| c2:importable_to pspec t2 |}
+  s1 s2
+  {| c1:exportable_from pspec t1 s1 |}
+  {| c2:importable_to pspec t2 s2 |}
   (pre:(t1 -> st_pre))
   (post:(x:t1 -> h0:heap -> st_post' (resexn t2) (pre x h0)))
-  (_:squash (forall (x:t1) h0. pre x h0 ==> pre_targetlang_arrow pspec #_ #c1.c_styp x h0))
-  (_:squash (forall (x:t1) h0 e h1. pre x h0 /\ post_targetlang_arrow pspec #_ #(witnessable_sum t2 err #c2.c_styp) h0 (Inr e) h1 ==> post x h0 (Inr e) h1))
-  (capture_check:select_check pspec t1 (resexn t2) #(witnessable_sum _ err #c2.c_styp) pre post)
-  : safe_importable_to pspec (x:t1 -> ST (resexn t2) (pre x) (post x)) = {
+ // (_:squash (forall (x:t1) h0. pre x h0 ==> pre_targetlang_arrow pspec #_ #c1.c_styp x h0))
+//  (_:squash (forall (x:t1) h0 e h1. pre x h0 /\ post_targetlang_arrow pspec #_ #(witnessable_sum t2 err #c2.c_styp) h0 (Inr e) h1 ==> post x h0 (Inr e) h1))
+//  (capture_check:select_check pspec t1 (resexn t2) #(witnessable_sum _ err #c2.c_styp) pre post)
+  : safe_importable_to pspec (x:t1 -> ST (resexn t2) (pre x) (post x)) (Node (Spec t1 c1.c_styp pre t2 c2.c_styp post) s1 s2) = {
   c_styp = witnessable_arrow t1 (resexn t2) pre post;
-  ityp = mk_targetlang_arrow pspec c1.ityp #c1.c_ityp.wt (resexn c2.ityp) #(witnessable_sum c2.ityp err #c2.c_ityp.wt);
+  ityp = mk_targetlang_arrow pspec c1.ityp #c1.c_ityp.wt (resexn c2.ityp) #(witnessable_resexn #c2.ityp #c2.c_ityp.wt);
   c_ityp = targetlang_arrow _ c1.ityp (resexn c2.ityp) #_ #(targetlang_sum _ c2.ityp err #c2.c_ityp);
-  safe_import = (fun (f:mk_targetlang_arrow pspec c1.ityp #c1.c_ityp.wt (resexn c2.ityp) #(witnessable_sum c2.ityp err #c2.c_ityp.wt)) (x:t1) ->
-    c1.lemma_export_preserves_prref x (Mktuple3?._2 pspec);
-    let (| _, check |) = capture_check x in
-    let x' = c1.export x in
-    let res : resexn c2.ityp = f x' in
-    let fres = (safe_importable_resexn pspec t2).safe_import res in
-    (safe_importable_resexn pspec t2).lemma_safe_import_preserves_prref res (Mktuple3?._2 pspec);
-    match check fres with
-    | Inl _ -> fres
-    | Inr err -> Inr err
+  safe_import = (fun (f:mk_targetlang_arrow pspec c1.ityp #c1.c_ityp.wt (resexn c2.ityp) #(witnessable_sum c2.ityp err #c2.c_ityp.wt)) (hocs:hoc_tree _) (x:t1) ->
+    let Node (| _, myhoc |) lhs rhs : hoc_tree _ = hocs in
+    match myhoc with
+    | EnforcePost c_pre c_post check -> begin
+      c_pre x;
+      c1.lemma_export_preserves_prref x (Mktuple3?._2 pspec) lhs;
+      let (| _, cb_check |) = check x in
+      let x' = c1.export lhs x in
+      let res : resexn c2.ityp = f x' in
+      let fres = (safe_importable_resexn pspec t2 s2).safe_import res (EmptyNode rhs Leaf) in
+      (safe_importable_resexn pspec t2 s2).lemma_safe_import_preserves_prref res (Mktuple3?._2 pspec) (EmptyNode rhs Leaf);
+      match cb_check fres with
+      | Inl _ -> fres
+      | Inr err -> (c_post x err; (Inr err))
+    end
+    | EnforcePre _ _ -> (admit (); (** no c_post? **) Inr (Contract_failure "Wrong contract!")) (** TODO: get rid off! **)
   );
-  lemma_safe_import_preserves_prref = (fun _ _ -> ())
+  lemma_safe_import_preserves_prref = (fun _ _ _ -> ())
 }
 
 instance safe_importable_arrow_safe
