state/SpecTree.fst
@@ -15,6 +15,9 @@ instance witnessable_err : witnessable err = {
   satisfy = (fun _ _ -> True);
 }
 
+instance witnessable_resexn #t {| witnessable t |} : witnessable (resexn t) =
+  witnessable_sum t err
+
 (** **** Tree **)
 type tree (a: Type) =
   | Leaf : tree a
@@ -106,50 +109,28 @@ type pck_spec (pspec:targetlang_pspec) =
     wt_argt:witnessable argt ->
     pre:(argt -> st_pre) ->
     rett:Type u#b ->
-    wt_rett:witnessable (resexn rett) ->
+    wt_rett:witnessable rett ->
     (post:(x:argt -> h0:heap -> st_post' (resexn rett) (pre x h0)))
     -> pck_spec pspec
 
 
 noeq
 type hoc pspec (s:pck_spec pspec) =
-(**| TrivialPre :
-    argt:Type u#a ->
-    wt_argt:witnessable argt ->
-    pre:(argt -> st_pre) ->
-    c_pre:squash (forall x h0. pre_targetlang_arrow pspec #argt #wt_argt x h0 ==> pre x h0) ->
-    rett:Type u#b ->
-    wt_rett:witnessable rett ->
-    (post:(x:argt -> h0:heap -> st_post' rett (pre x h0))) ->
-    c_post:(squash (forall x h0 r h1. post x h0 r h1 ==> post_targetlang_arrow pspec #rett #wt_rett h0 r h1))
-    -> pck_hoc pspec **)
-
 | EnforcePre :
     check:(select_check pspec (Spec?.argt s) unit
                         (pre_targetlang_arrow pspec #(Spec?.argt s) #(Spec?.wt_argt s))
                         (fun x _ _ h1 -> (Spec?.pre s) x h1)) ->
-    c_post:(squash (forall x h0 r h1. (Spec?.post s) x h0 r h1 ==> post_targetlang_arrow pspec #(resexn (Spec?.rett s)) #(Spec?.wt_rett s) h0 r h1))
+    c_post:(x:(Spec?.argt s) -> r:(resexn (Spec?.rett s)) -> Lemma (forall h0 h1. (Spec?.post s) x h0 r h1 ==> post_targetlang_arrow pspec #(resexn (Spec?.rett s)) #(witnessable_resexn #_ #(Spec?.wt_rett s)) h0 r h1))
     -> hoc pspec s
-
-(**| TrivialPost :
-    argt:Type u#a ->
-    wt_argt:witnessable argt ->
-    pre:(argt -> st_pre) ->
-    c_pre:squash (forall x h0. pre x h0 ==> pre_targetlang_arrow pspec #argt #wt_argt x h0) ->
-    rett:Type u#b ->
-    wt_rett:witnessable rett ->
-    post:(x:argt -> h0:heap -> st_post' rett (pre x h0)) ->
-    c_post:(squash (forall x h0 r h1. post_targetlang_arrow pspec #rett #wt_rett h0 r h1 ==> post x h0 r h1))
-    -> pck_hoc pspec **)
 
 | EnforcePost :
-    c_pre:squash (forall x h0. (Spec?.pre s) x h0 ==> pre_targetlang_arrow pspec #(Spec?.argt s) #(Spec?.wt_argt s) x h0) ->
-    c_post:(squash (forall x h0 e h1. (Spec?.post s) x h0 (Inr e) h1 ==>
-                      post_targetlang_arrow pspec #(resexn (Spec?.rett s)) #(Spec?.wt_rett s) h0 (Inr e) h1)) ->
-    check:(select_check pspec (Spec?.argt s) (resexn (Spec?.rett s)) #(Spec?.wt_rett s) (Spec?.pre s) (Spec?.post s))
+    c_pre:(x:(Spec?.argt s) -> Lemma (forall h0. (Spec?.pre s) x h0 ==> pre_targetlang_arrow pspec #(Spec?.argt s) #(Spec?.wt_argt s) x h0)) ->
+    c_post:(x:(Spec?.argt s) -> e:err -> Lemma (forall h0 h1. (Spec?.pre s) x h0 /\ post_targetlang_arrow pspec #_ #(witnessable_resexn #_ #(Spec?.wt_rett s)) h0 (Inr e) h1 ==> (Spec?.post s) x h0 (Inr e) h1)) ->
+    check:(select_check pspec (Spec?.argt s) (resexn (Spec?.rett s)) #(witnessable_resexn #_ #(Spec?.wt_rett s)) (Spec?.pre s) (Spec?.post s))
     -> hoc pspec s
 
-type pck_hoc pspec = s:pck_spec pspec & hoc pspec s
+type pck_hoc pspec =
+  s:pck_spec pspec & (hoc pspec s)
 
 private
 let myspec : pck_spec concrete_spec =
@@ -158,7 +139,7 @@ let myspec : pck_spec concrete_spec =
     (witnessable_ref int)
     (fun x h -> sel h x > 5)
     unit
-    (witnessable_sum unit err #witnessable_unit #witnessable_err)
+    witnessable_unit
     (fun _ -> post_targetlang_arrow concrete_spec)
 
 private
@@ -175,7 +156,7 @@ let test_pre : hoc concrete_spec myspec =
           else Inr (Contract_failure "less than 5")
       ) in
       (| eh0, check |))
-    ()
+    (fun _ _ -> ())
 
 private
 let myspec' : pck_spec concrete_spec =
@@ -184,18 +165,18 @@ let myspec' : pck_spec concrete_spec =
     (witnessable_ref int)
     (pre_targetlang_arrow concrete_spec)
     unit
-    (witnessable_sum unit err #witnessable_unit #witnessable_err)
-    (fun x h0 r h1 -> sel h1 x > 5 /\ post_targetlang_arrow concrete_spec h0 r h1)
+    witnessable_unit
+    (fun x h0 r h1 -> (Inr? r \/ sel h1 x > 5) /\ post_targetlang_arrow concrete_spec h0 r h1)
 
 private
 let test_post : hoc concrete_spec myspec' =
   EnforcePost
-    ()
-    ()
+    (fun _ -> ())
+    (fun _ _ -> ())
     (fun x ->
       let x : ref int = x in
       let eh0 = get_heap () in
-      let check : cb_check concrete_spec (ref int) (resexn unit) #(Spec?.wt_rett myspec') (Spec?.pre myspec') (Spec?.post myspec') x eh0 = (
+      let check : cb_check concrete_spec (ref int) (resexn unit) #(witnessable_resexn #_ #(Spec?.wt_rett myspec')) (Spec?.pre myspec') (Spec?.post myspec') x eh0 = (
         fun _ ->
           assert (witnessed (contains_pred x));
           recall (contains_pred x);
@@ -205,5 +186,5 @@ let test_post : hoc concrete_spec myspec' =
       (| eh0, check |))
 
 let spec_tree pspec = tree (pck_spec pspec)
-let hoc_tree pspec (st:spec_tree pspec) =
+let hoc_tree #pspec (st:spec_tree pspec) =
   hocs:(tree (pck_hoc pspec)){equal_trees st (map_tree hocs dfst)}
